split up the Bucket into Bucket and BucketMap

lib/Buckets/BucketWeights.i.dfy
@@ -26,6 +26,7 @@ module BucketWeights {
   import opened BucketsLib
   import opened NativeTypes
   import opened KeyType
+  import opened BucketMaps
   import MSets = Multisets
 
   
@@ -44,81 +45,12 @@ module BucketWeights {
     }
   }
 
-  lemma MergeGainsNoWeight(parent: Message, child: Message)
-  ensures WeightMessage(Merge(parent, child)) <= WeightMessage(parent) + WeightMessage(child)
-  {
-    //var merged := Merge(parent, child);
-    //if (parent.Update? && child.Define?) {
-    //}
-  }
-
-  function method WeightKeyUint64(key: Key) : (w:uint64)
-  ensures w as int == WeightKey(key)
-  {
-    4 + |key| as uint64
-  }
-
-  function method WeightMessageUint64(msg: Message) : (w:uint64)
-  ensures w as int == WeightMessage(msg)
-  {
-    match msg {
-      case Define(value) => 4 + |value| as uint64
-      case Update(delta) => 0
-    }
-  }
-
   function {:opaque} WeightKeyMultiset(keys: multiset<Key>) : (result: nat)
     ensures |keys| == 0 ==> result == 0
   {
     var weights := MSets.Apply(WeightKey, keys);
     assert |keys| == 0 ==> |weights| == 0;
     MSets.FoldSimple<nat>(0, MSets.AddNat, weights)
-  }
-
-  function {:opaque} WeightKeySeq(keys: seq<Key>) : nat
-  {
-    var weights := ApplyOpaque(WeightKey, keys);
-    FoldFromRight<nat, nat>(MSets.AddNat, 0, weights)
-  }
-
-  lemma WeightKeyMultisetAdditive(things1: multiset<Key>, things2: multiset<Key>)
-    ensures WeightKeyMultiset(things1 + things2) == WeightKeyMultiset(things1) + WeightKeyMultiset(things2)
-  {
-    var weights1 := MSets.Apply(WeightKey, things1);
-    var weights2 := MSets.Apply(WeightKey, things2);
-    MSets.ApplyAdditive(WeightKey, things1, things2);
-    MSets.reveal_IsIdentity();
-    MSets.reveal_IsAssociative();
-    MSets.reveal_IsCommutative();
-    MSets.FoldSimpleAdditive<nat>(0, MSets.AddNat, weights1, weights2);
-    reveal_WeightKeyMultiset();
-  }
-
-  lemma WeightKeyMultisetUpperBound(keys: multiset<Key>)
-    ensures WeightKeyMultiset(keys) <= |keys| * (4 + KeyType.MaxLen() as nat)
-  {
-    if |keys| == 0 {
-    } else {
-      var key :| key in keys;
-      var rest := keys - multiset{key};
-      assert keys == rest + multiset{key};
-      calc <= {
-        WeightKeyMultiset(keys);
-        //WeightKeyMultiset(rest + multiset{key});
-        { WeightKeyMultisetAdditive(rest, multiset{key}); }
-        WeightKeyMultiset(rest) + WeightKeyMultiset(multiset{key});
-        { WeightKeyMultisetUpperBound(rest); }
-        |rest| * (4 + KeyType.MaxLen() as nat) + WeightKeyMultiset(multiset{key});
-        {
-          reveal_WeightKeyMultiset();
-          MSets.ApplySingleton(WeightKey, key);
-          MSets.FoldSimpleSingleton<nat>(0, MSets.AddNat, WeightKey(key));
-        }
-        //|rest| * (4 + KeyType.MaxLen() as nat) + WeightKey(key);
-        //|rest| * (4 + KeyType.MaxLen() as nat) + (4 + KeyType.MaxLen() as nat);
-        |keys| * (4 + KeyType.MaxLen() as nat );
-      }
-    }
   }
 
   function {:opaque} WeightMessageMultiset(msgs: multiset<Message>) : (result: nat)
@@ -128,26 +60,7 @@ module BucketWeights {
     assert |msgs| == 0 ==> |weights| == 0;
     MSets.FoldSimple<nat>(0, MSets.AddNat, weights)
   }
-  
-  function {:opaque} WeightMessageSeq(msgs: seq<Message>) : nat
-  {
-    var weights := ApplyOpaque(WeightMessage, msgs);
-    FoldFromRight<nat, nat>(MSets.AddNat, 0, weights)
-  }
-
-  lemma WeightMessageMultisetAdditive(things1: multiset<Message>, things2: multiset<Message>)
-    ensures WeightMessageMultiset(things1 + things2) == WeightMessageMultiset(things1) + WeightMessageMultiset(things2)
-  {
-    var weights1 := MSets.Apply(WeightMessage, things1);
-    var weights2 := MSets.Apply(WeightMessage, things2);
-    MSets.ApplyAdditive(WeightMessage, things1, things2);
-    MSets.reveal_IsIdentity();
-    MSets.reveal_IsAssociative();
-    MSets.reveal_IsCommutative();
-    MSets.FoldSimpleAdditive<nat>(0, MSets.AddNat, weights1, weights2);
-    reveal_WeightMessageMultiset();
-  }
-  
+ 
   function WeightKeyList(keys: seq<Key>) : (result: nat)
     ensures |keys| == 0 ==> result == 0
   {
@@ -174,7 +87,51 @@ module BucketWeights {
     )
   }
 
-  
+  function {:opaque} WeightBucketMap(m: BucketMap) : (w: nat)
+  {
+    WeightKeyMultiset(multiset(m.Keys)) + WeightMessageMultiset(Multisets.ValueMultiset(m))
+  }
+
+  function method WeightKeyUint64(key: Key) : (w:uint64)
+  ensures w as int == WeightKey(key)
+  {
+    4 + |key| as uint64
+  }
+
+  function method WeightMessageUint64(msg: Message) : (w:uint64)
+  ensures w as int == WeightMessage(msg)
+  {
+    match msg {
+      case Define(value) => 4 + |value| as uint64
+      case Update(delta) => 0
+    }
+  }
+
+  lemma WeightKeyMultisetAdditive(things1: multiset<Key>, things2: multiset<Key>)
+    ensures WeightKeyMultiset(things1 + things2) == WeightKeyMultiset(things1) + WeightKeyMultiset(things2)
+  {
+    var weights1 := MSets.Apply(WeightKey, things1);
+    var weights2 := MSets.Apply(WeightKey, things2);
+    MSets.ApplyAdditive(WeightKey, things1, things2);
+    MSets.reveal_IsIdentity();
+    MSets.reveal_IsAssociative();
+    MSets.reveal_IsCommutative();
+    MSets.FoldSimpleAdditive<nat>(0, MSets.AddNat, weights1, weights2);
+    reveal_WeightKeyMultiset();
+  }
+
+  lemma WeightMessageMultisetAdditive(things1: multiset<Message>, things2: multiset<Message>)
+    ensures WeightMessageMultiset(things1 + things2) == WeightMessageMultiset(things1) + WeightMessageMultiset(things2)
+  {
+    var weights1 := MSets.Apply(WeightMessage, things1);
+    var weights2 := MSets.Apply(WeightMessage, things2);
+    MSets.ApplyAdditive(WeightMessage, things1, things2);
+    MSets.reveal_IsIdentity();
+    MSets.reveal_IsAssociative();
+    MSets.reveal_IsCommutative();
+    MSets.FoldSimpleAdditive<nat>(0, MSets.AddNat, weights1, weights2);
+    reveal_WeightMessageMultiset();
+  }
   
   lemma WeightKeyListFlatten(keys: seq<Key>)
     ensures WeightKeyList(keys) == FlattenLength(FlattenShape(keys)) + 4 * |keys|
@@ -205,46 +162,8 @@ module BucketWeights {
     }
   }
 
-  lemma WeightKeySeqList(keys: seq<Key>)
-    ensures WeightKeySeq(keys) == WeightKeyList(keys)
-  {
-    var ws := ApplyOpaque(WeightKey, keys);
-    var ws' := MSets.Apply(WeightKey, multiset(keys));
-    calc {
-      WeightKeySeq(keys);
-      { reveal_WeightKeySeq(); }
-      FoldFromRight<nat, nat>(MSets.AddNat, 0, ws);
-      { MSets.natsumProperties(); }
-      { MSets.FoldSeq<nat>(0, MSets.AddNat, ws); }
-      MSets.FoldSimple<nat>(0, MSets.AddNat, multiset(ws));
-      { MSets.ApplySeq(WeightKey, keys); }
-      MSets.FoldSimple<nat>(0, MSets.AddNat, ws');
-      { reveal_WeightKeyMultiset(); }
-      WeightKeyList(keys);
-    }
-  }
-
-  lemma WeightMessageSeqList(msgs: seq<Message>)
-    ensures WeightMessageSeq(msgs) == WeightMessageList(msgs)
-  {
-    var ws := ApplyOpaque(WeightMessage, msgs);
-    var ws' := MSets.Apply(WeightMessage, multiset(msgs));
-    calc {
-      WeightMessageSeq(msgs);
-      { reveal_WeightMessageSeq(); }
-      FoldFromRight<nat, nat>(MSets.AddNat, 0, ws);
-      { MSets.natsumProperties(); }
-      { MSets.FoldSeq<nat>(0, MSets.AddNat, ws); }
-      MSets.FoldSimple<nat>(0, MSets.AddNat, multiset(ws));
-      { MSets.ApplySeq(WeightMessage, msgs); }
-      MSets.FoldSimple<nat>(0, MSets.AddNat, ws');
-      { reveal_WeightMessageMultiset(); }
-      WeightMessageList(msgs);
-    }
-  }
-
   lemma WeightBucketEmpty()
-  ensures WeightBucket(B(map[])) == 0
+  ensures WeightBucket(EmptyBucket()) == 0
   {
   }
 
@@ -272,452 +191,192 @@ module BucketWeights {
     WeightMessageSingleton(msg);
   }
 
-  lemma WeightWellMarshalledLe(unsorted: Bucket, sorted: Bucket)
+  // when going seqs -> map, weight might decrease if there are dupe keys
+  lemma Weight_BucketMap_le_Bucket(b: Bucket)
+  requires PreWFBucket(b)
+  ensures WeightBucketMap(b.as_map()) <= WeightBucket(b)
+  {
+    var m := b.as_map();
+    MapSeqs.lemma_multisets_le(b.keys, b.msgs);
+    assert WeightKeyMultiset(multiset(m.Keys)) <= WeightKeyMultiset(multiset(b.keys)) by {
+      var x := multiset(b.keys) - multiset(m.Keys);
+      assert multiset(m.Keys) + x == multiset(b.keys);
+      WeightKeyMultisetAdditive(multiset(m.Keys), x);
+    }
+    assert WeightMessageMultiset(Multisets.ValueMultiset(m))
+        <= WeightMessageMultiset(multiset(b.msgs)) by {
+      var x := multiset(b.msgs) - Multisets.ValueMultiset(m);
+      assert Multisets.ValueMultiset(m) + x == multiset(b.msgs);
+      WeightMessageMultisetAdditive(Multisets.ValueMultiset(m), x);
+    }
+    reveal_WeightBucketMap();
+  }
+
+  // but seqs -> map preserves the 'weight' if the input keys are sorted
+  lemma Weight_BucketMap_eq_Bucket(b: Bucket)
+  requires PreWFBucket(b)
+  requires IsStrictlySorted(b.keys)
+  ensures WeightBucketMap(b.as_map()) == WeightBucket(b)
+  {
+    Weight_Bucket_eq_BucketMap(b.as_map());
+    B_of_as_map_sorted(b);
+  }
+
+  // going from map -> seqs preserves weights
+  lemma Weight_Bucket_eq_BucketMap(m: BucketMap)
+  ensures WeightBucket(B(m)) == WeightBucketMap(m)
+  {
+    var b := B(m);
+    assert MapSeqs.map_of_seqs(b.keys, b.msgs) == m;
+    MapSeqs.lemma_multisets_eq(b.keys, b.msgs);
+    reveal_WeightBucketMap();
+  }
+
+  lemma Weight_SortedBucket_le_UnsortedBucket(unsorted: Bucket, sorted: Bucket)
     requires PreWFBucket(unsorted)
     requires PreWFBucket(sorted)
     requires BucketWellMarshalled(sorted)
-    requires unsorted.b == sorted.b
+    requires unsorted.as_map() == sorted.as_map()
     ensures WeightBucket(sorted) <= WeightBucket(unsorted)
   {
-    WellMarshalledKeyMultiset(sorted);
-    //assert multiset(sorted.keys) <= multiset(unsorted.keys);
-    WeightKeyMultisetAdditive(multiset(sorted.keys), multiset(unsorted.keys) - multiset(sorted.keys));
-    assert multiset(unsorted.keys) == multiset(sorted.keys) + (multiset(unsorted.keys) - multiset(sorted.keys));
-    
-    WFMessageMultiset(sorted);
-    WFMessageMultiset(unsorted);
-    //assert multiset(sorted.msgs) <= multiset(unsorted.msgs);
-    WeightMessageMultisetAdditive(multiset(sorted.msgs), multiset(unsorted.msgs) - multiset(sorted.msgs));
-    assert multiset(unsorted.msgs) == multiset(sorted.msgs) + (multiset(unsorted.msgs) - multiset(sorted.msgs));
+    calc <= {
+      WeightBucket(sorted);
+      {
+        assert B(sorted.as_map()).as_map() == sorted.as_map();
+        MapSeqs.SeqsEqOfMapsEq(sorted.keys, sorted.msgs,
+            B(sorted.as_map()).keys,
+            B(sorted.as_map()).msgs);
+        assert sorted == B(sorted.as_map());
+      }
+      WeightBucket(B(sorted.as_map()));
+      {
+        Weight_Bucket_eq_BucketMap(sorted.as_map());
+      }
+      WeightBucketMap(sorted.as_map());
+      {
+        Weight_BucketMap_le_Bucket(unsorted);
+      }
+      WeightBucket(unsorted);
+    }
   }
 
-  lemma WeightWellMarshalledSubsetLe(smaller: Bucket, larger: Bucket)
-    requires PreWFBucket(smaller)
-    requires PreWFBucket(larger)
-    requires BucketWellMarshalled(smaller)
-    requires smaller.b.Keys <= larger.b.Keys
-    requires forall k | k in smaller.b.Keys :: smaller.b[k] == larger.b[k];
-    ensures WeightBucket(smaller) <= WeightBucket(larger)
+  lemma WeightBucketMapSubsetLe(smaller: BucketMap, larger: BucketMap)
+    requires smaller.Keys <= larger.Keys
+    requires forall k | k in smaller.Keys :: smaller[k] == larger[k];
+    ensures WeightBucketMap(smaller) <= WeightBucketMap(larger)
   {
-    WellMarshalledKeyMultiset(smaller);
-    assert multiset(larger.keys) == multiset(smaller.keys) + (multiset(larger.keys) - multiset(smaller.keys));
-    WeightKeyMultisetAdditive(multiset(smaller.keys), multiset(larger.keys) - multiset(smaller.keys));
+    calc <= {
+      WeightKeyMultiset(multiset(smaller.Keys));
+      {
+        assert multiset(larger.Keys) == multiset(smaller.Keys) + (multiset(larger.Keys) - multiset(smaller.Keys));
+        WeightKeyMultisetAdditive(multiset(smaller.Keys), multiset(larger.Keys) - multiset(smaller.Keys));
+      }
+      WeightKeyMultiset(multiset(larger.Keys));
+    }
 
     calc <= {
-      multiset(smaller.msgs);
-      { WFMessageMultiset(smaller); }
-      Multisets.ValueMultiset(smaller.b);
-      //MSets.Apply(MSets.ValueMultisetFn(smaller.b), multiset(smaller.b.Keys));
-      { MSets.ApplyEquivalentFns(MSets.ValueMultisetFn(smaller.b), MSets.ValueMultisetFn(larger.b), multiset(smaller.b.Keys)); }
-      MSets.Apply(MSets.ValueMultisetFn(larger.b), multiset(smaller.b.Keys));
-      { MSets.ApplyMonotonic(MSets.ValueMultisetFn(larger.b), multiset(smaller.b.Keys), multiset(larger.b.Keys)); }
-      MSets.Apply(MSets.ValueMultisetFn(larger.b), multiset(larger.b.Keys));
-      { WFMessageMultiset(larger); }
-      multiset(larger.msgs);
+      WeightMessageMultiset(Multisets.ValueMultiset(smaller));
+      {
+        calc <= {
+          Multisets.ValueMultiset(smaller);
+          //MSets.Apply(MSets.ValueMultisetFn(smaller), multiset(smaller.Keys));
+          { MSets.ApplyEquivalentFns(MSets.ValueMultisetFn(smaller), MSets.ValueMultisetFn(larger), multiset(smaller.Keys)); }
+          MSets.Apply(MSets.ValueMultisetFn(larger), multiset(smaller.Keys));
+          { MSets.ApplyMonotonic(MSets.ValueMultisetFn(larger), multiset(smaller.Keys), multiset(larger.Keys)); }
+          MSets.Apply(MSets.ValueMultisetFn(larger), multiset(larger.Keys));
+          Multisets.ValueMultiset(larger);
+        }
+        assert Multisets.ValueMultiset(larger) == Multisets.ValueMultiset(smaller) + (Multisets.ValueMultiset(larger) - Multisets.ValueMultiset(smaller));
+        WeightMessageMultisetAdditive(Multisets.ValueMultiset(smaller), Multisets.ValueMultiset(larger) - Multisets.ValueMultiset(smaller));
+      }
+      WeightMessageMultiset(Multisets.ValueMultiset(larger));
     }
-    assert multiset(larger.msgs) == multiset(smaller.msgs) + (multiset(larger.msgs) - multiset(smaller.msgs));
-    WeightMessageMultisetAdditive(multiset(smaller.msgs), multiset(larger.msgs) - multiset(smaller.msgs));
-  }
-  
-  lemma WeightWellMarshalledListPointwiseLe(blist: BucketList, blist': BucketList)
-    requires |blist| == |blist'|
-    requires forall i | 0 <= i < |blist| :: PreWFBucket(blist[i])
-    requires forall i | 0 <= i < |blist| :: PreWFBucket(blist'[i])
-    requires forall i | 0 <= i < |blist| :: WeightBucket(blist'[i]) <= WeightBucket(blist[i])
-    //requires forall i | 0 <= i < |blist| :: blist[i] == blist'[i] || BucketWellMarshalled(blist'[i])
-    ensures WeightBucketList(blist') <= WeightBucketList(blist)
-  {
-    if |blist| == 0 {
-    } else {
-      WeightWellMarshalledListPointwiseLe(DropLast(blist), DropLast(blist'));
-      assert blist == DropLast(blist) + [ Last(blist) ];
-      assert blist' == DropLast(blist') + [ Last(blist') ];
-      WeightBucketListConcatOne(DropLast(blist), Last(blist));
-      WeightBucketListConcatOne(DropLast(blist'), Last(blist'));
-    }
-  }
-    
-  // Commonly-used filters for Image()
-  function AllKeys() : iset<Key>
-  {
-    iset k | true
-  }
-  function IncludeKey(key:Key) : iset<Key>
-  {
-    iset k | k == key
-  }
-  function ExcludeKey(key:Key) : iset<Key>
-  {
-    iset k | k != key
+
+    reveal_WeightBucketMap();
   }
 
-  // Image of bucket showing only keys in filter.
-  function {:opaque} Image(bucket:Bucket, filter:iset<Key>) : (image:Bucket)
-    ensures BucketWellMarshalled(image)
-    ensures PreWFBucket(image)
-    ensures |image.keys| == |image.msgs|
-    ensures WFBucketMap(bucket.b) ==> WFBucket(image)
+  lemma WeightBucketInduct(bucket: BucketMap, key: Key, msg: Message)
+    requires key !in bucket
+    ensures WeightBucketMap(bucket[key := msg]) == WeightBucketMap(bucket) + WeightKey(key) + WeightMessage(msg)
   {
-    B(map k | k in bucket.b && k in filter :: bucket.b[k])
-  }
-
-  lemma ImageShape(b:Bucket, s:iset<Key>)
-    ensures forall k :: k in b.b && k in s <==> k in Image(b, s).b.Keys
-    ensures forall k :: k in Image(b,s).b ==> Image(b,s).b[k] == b.b[k];
-  {
-    reveal_Image();
-  }
-
-  lemma ImageMapIdentity(bucket:Bucket, s:iset<Key>)
-    requires forall k :: k in bucket.b ==> k in s
-    ensures bucket.b == Image(bucket, s).b
-  {
-    reveal_Image();
-  }
-  
-  lemma ImageIdentity(bucket:Bucket, s:iset<Key>)
-  requires PreWFBucket(bucket)
-  requires BucketWellMarshalled(bucket)
-  requires forall k :: k in bucket.b ==> k in s
-  ensures bucket == Image(bucket, s)
-  {
-    ImageMapIdentity(bucket, s);
-    WellMarshalledBucketsEq(bucket, Image(bucket, s));
-  }
-
-  lemma ImageTrim(bucket:Bucket, s:iset<Key>, trimBucket:Bucket)
-    requires forall k :: k in trimBucket.b <==> k in bucket.b && k in s
-    requires forall k :: k in trimBucket.b ==> trimBucket.b[k] == bucket.b[k]
-    ensures Image(bucket, s).b == trimBucket.b
-  {
-    ImageShape(bucket, s);
-  }
-
-  lemma ImageEquiv(a:Bucket, b:Bucket, s:iset<Key>)
-    requires forall k :: k in a.b.Keys && k in s <==> k in b.b.Keys && k in s
-    requires forall k :: k in a.b.Keys && k in s ==> a.b[k] == b.b[k]
-    ensures Image(a, s) == Image(b, s)
-  {
-    reveal_Image();
-  }
-
-
-  lemma ImageSubset(b:Bucket, s:iset<Key>, t:iset<Key>)
-    requires s <= t;
-    ensures Image(Image(b, t), s) == Image(b, s)
-    ensures Image(b, s).b.Keys <= Image(b, t).b.Keys
-  {
-    reveal_Image();
-  }
-
-  lemma ImageIntersect(b:Bucket, s:iset<Key>, t:iset<Key>)
-    ensures Image(Image(b, s), t) == Image(b, s * t)
-  {
-    reveal_Image();
-  }
-
-  // used internally
-  lemma ImageSplitsKeys(bucket:Bucket, a:iset<Key>, b:iset<Key>)
-    requires PreWFBucket(bucket)
-    requires BucketWellMarshalled(bucket)
-    requires a !! b
-    requires forall k:Key :: k in bucket.b ==> k in a + b
-    ensures multiset(bucket.keys) == multiset(Image(bucket, a).keys) + multiset(Image(bucket, b).keys)
-  {
-    var abucket := Image(bucket, a);
-    var bbucket := Image(bucket, b);
-    
     calc {
-      multiset(bucket.keys);
-      { WellMarshalledKeyMultiset(bucket); }
-      multiset(bucket.b.Keys);
-      { reveal_Image(); }
-      multiset(abucket.b.Keys) + multiset(bbucket.b.Keys);
+      WeightKeyMultiset(multiset(bucket[key := msg].Keys));
       {
-        WellMarshalledKeyMultiset(abucket);
-        WellMarshalledKeyMultiset(bbucket);
+        calc {
+          multiset(bucket[key := msg].Keys);
+          multiset(bucket.Keys) + multiset{key};
+        }
+        WeightKeyMultisetAdditive(multiset(bucket.Keys), multiset{key});
+        WeightKeySingleton(key);
+        //assert WeightKeyMultiset(multiset{key}) == WeightKey(key);
       }
-      multiset(Image(bucket, a).keys) + multiset(Image(bucket, b).keys);
+      WeightKeyMultiset(multiset(bucket.Keys)) + WeightKey(key);
     }
-  }
 
-  // used internally
-  lemma ImageSplitsMessages(bucket:Bucket, a:iset<Key>, b:iset<Key>)
-    requires PreWFBucket(bucket)
-    requires BucketWellMarshalled(bucket)
-    requires a !! b
-    requires forall k:Key :: k in bucket.b ==> k in a + b
-    ensures multiset(bucket.msgs) == multiset(Image(bucket, a).msgs) + multiset(Image(bucket, b).msgs)
-  {
-    var abucket := Image(bucket, a);
-    var bbucket := Image(bucket, b);
-
-    var fn := Multisets.ValueMultisetFn(bucket.b);
-    var afn := Multisets.ValueMultisetFn(abucket.b);
-    var bfn := Multisets.ValueMultisetFn(bbucket.b);
-    
     calc {
-      multiset(bucket.msgs);
-      { WFMessageMultiset(bucket); }
-      Multisets.ValueMultiset(bucket.b);
-      Multisets.Apply(fn, multiset(bucket.b.Keys));
-      { WellMarshalledKeyMultiset(bucket); }
-      Multisets.Apply(fn, multiset(bucket.keys));
+      WeightMessageMultiset(Multisets.ValueMultiset(bucket[key := msg]));
       {
-        ImageSplitsKeys(bucket, a, b);
-        Multisets.ApplyAdditive(fn, multiset(abucket.keys), multiset(bbucket.keys));
+        calc {
+          Multisets.ValueMultiset(bucket[key := msg]);
+          {
+            Multisets.ValueMultisetInduct(bucket, key, msg);
+          }
+          Multisets.ValueMultiset(bucket) + multiset{msg};
+        }
+        WeightMessageMultisetAdditive(Multisets.ValueMultiset(bucket), multiset{msg});
+        WeightMessageSingleton(msg);
       }
-      Multisets.Apply(fn, multiset(abucket.keys)) + Multisets.Apply(fn, multiset(bbucket.keys));
-      {
-        WellMarshalledKeyMultiset(abucket);
-        WellMarshalledKeyMultiset(bbucket);
-      }
-      Multisets.Apply(fn, multiset(abucket.b.Keys)) + Multisets.Apply(fn, multiset(bbucket.b.Keys));
-      {
-        reveal_Image();
-        Multisets.ApplyEquivalentFns(fn, afn, multiset(abucket.b.Keys));
-        Multisets.ApplyEquivalentFns(fn, bfn, multiset(bbucket.b.Keys));
-      }
-      Multisets.ValueMultiset(abucket.b) + Multisets.ValueMultiset(bbucket.b);
-      {
-        WFMessageMultiset(abucket);
-        WFMessageMultiset(bbucket);
-      }
-      multiset(abucket.msgs) + multiset(bbucket.msgs);
+      WeightMessageMultiset(Multisets.ValueMultiset(bucket)) + WeightMessage(msg);
     }
+
+    reveal_WeightBucketMap();
   }
 
   // used internally
-  lemma WeightBucketLinearInKeySet(bucket:Bucket, a:iset<Key>, b:iset<Key>)
-  requires PreWFBucket(bucket)
-  requires BucketWellMarshalled(bucket)
-  requires a !! b
-  requires forall k:Key :: k in bucket.b ==> k in a + b
-  ensures WeightBucket(bucket) == WeightBucket(Image(bucket, a)) + WeightBucket(Image(bucket, b))
-  decreases |Image(bucket, a).b.Keys| + |Image(bucket, b).b.Keys|, 1
-  {
-    var keys := bucket.keys;
-    var msgs := bucket.msgs;
-    var keysweights := MSets.Apply(WeightKey, multiset(keys));
-    var msgsweights := MSets.Apply(WeightMessage, multiset(msgs));
-
-    var akeys := Image(bucket, a).keys;
-    var amsgs := Image(bucket, a).msgs;
-    var ab := Image(bucket, a).b;
-    var akeysweights := MSets.Apply(WeightKey, multiset(akeys));
-    var amsgsweights := MSets.Apply(WeightMessage, multiset(amsgs));
-    
-    var bkeys := Image(bucket, b).keys;
-    var bmsgs := Image(bucket, b).msgs;
-    var bb := Image(bucket, b).b;
-    var bkeysweights := MSets.Apply(WeightKey, multiset(bkeys));
-    var bmsgsweights := MSets.Apply(WeightMessage, multiset(bmsgs));
-
-    Multisets.natsumProperties();
-    
-    calc {
-      WeightBucket(bucket);
-      // WeightKeyList(keys) + WeightMessageList(msgs);
-      // WeightKeyMultiset(multiset(keys)) + WeightMessageMultiset(multiset(msgs));
-      {
-        reveal_WeightKeyMultiset();
-        reveal_WeightMessageMultiset();
-      }
-      MSets.FoldSimple<nat>(0, MSets.AddNat, keysweights) + MSets.FoldSimple<nat>(0, MSets.AddNat, msgsweights);
-      {
-        ImageSplitsMessages(bucket, a, b);
-        //assert multiset(msgs) == multiset(amsgs) + multiset(bmsgs);
-        Multisets.ApplyAdditive(WeightMessage, multiset(amsgs), multiset(bmsgs));
-        //assert msgsweights == amsgsweights + bmsgsweights;
-        Multisets.FoldSimpleAdditive<nat>(0, MSets.AddNat, amsgsweights, bmsgsweights);
-      }
-        MSets.FoldSimple<nat>(0, MSets.AddNat, keysweights)
-      + MSets.FoldSimple<nat>(0, MSets.AddNat, amsgsweights) + MSets.FoldSimple<nat>(0, MSets.AddNat, bmsgsweights);
-      {
-        ImageSplitsKeys(bucket, a, b);
-        //assert multiset(keys) == multiset(akeys) + multiset(bkeys);
-        Multisets.ApplyAdditive(WeightKey, multiset(akeys), multiset(bkeys));
-        //assert keysweights == akeysweights + bkeysweights;
-        Multisets.FoldSimpleAdditive<nat>(0, MSets.AddNat, akeysweights, bkeysweights);
-      }
-        MSets.FoldSimple<nat>(0, MSets.AddNat, akeysweights) + MSets.FoldSimple<nat>(0, MSets.AddNat, amsgsweights)
-      + MSets.FoldSimple<nat>(0, MSets.AddNat, bkeysweights) + MSets.FoldSimple<nat>(0, MSets.AddNat, bmsgsweights);
-      {
-        reveal_WeightKeyMultiset();
-        reveal_WeightMessageMultiset();
-      }
-      //   WeightKeyMultiset(multiset(akeys)) + WeightMessageMultiset(multiset(amsgs))
-      // + WeightKeyMultiset(multiset(bkeys)) + WeightMessageMultiset(multiset(bmsgs));
-      //   WeightKeyList(akeys) + WeightMessageList(amsgs)
-      // + WeightKeyList(bkeys) + WeightMessageList(bmsgs);
-      WeightBucket(Image(bucket, a)) + WeightBucket(Image(bucket, b));
-    }
-  }
-
-  // A variant that's handy if a+b don't cover bucket.
-  // used internally
-  lemma WeightBucketLinearInKeySetSum(bucket:Bucket, a:iset<Key>, b:iset<Key>)
-    requires PreWFBucket(bucket)
-    requires BucketWellMarshalled(bucket)
-    requires a!!b
-    ensures WeightBucket(Image(bucket, a + b)) == WeightBucket(Image(bucket, a)) + WeightBucket(Image(bucket, b));
-  {
-    var c := a + b;
-    calc {
-      WeightBucket(Image(bucket, a))
-        + WeightBucket(Image(bucket, b));
-        { ImageSubset(bucket, b, c); }
-      WeightBucket(Image(bucket, a))
-        + WeightBucket(Image(Image(bucket, c), b));
-        { ImageSubset(bucket, a, c); }
-      WeightBucket(Image(Image(bucket, c), a))
-        + WeightBucket(Image(Image(bucket, c), b));
-      {
-        ImageShape(bucket, c);
-        WeightBucketLinearInKeySet(Image(bucket, c), a, b);
-      }
-      WeightBucket(Image(bucket, c));
-    }
-  }
-
-  function WeightOneKey(bucket: Bucket, key: Key) : (w:int)
-    requires PreWFBucket(bucket)
-    requires BucketWellMarshalled(bucket)
-  {
-    if key in bucket.b
-      then WeightKey(key) + WeightMessage(bucket.b[key])
-      else 0
-  }
-
-  // used internally
-  lemma KeyContribution(bucket: Bucket, key: Key)
-    requires PreWFBucket(bucket)
-    requires BucketWellMarshalled(bucket)
-    ensures WeightBucket(bucket) == WeightBucket(Image(bucket, ExcludeKey(key))) + WeightOneKey(bucket, key);
-  {
-    var kbucket := Image(bucket, IncludeKey(key));
-    
-    ImageIdentity(bucket, ExcludeKey(key) + IncludeKey(key));
-    WeightBucketLinearInKeySetSum(bucket, ExcludeKey(key), IncludeKey(key));
-
-    ImageShape(bucket, IncludeKey(key));
-    if key in bucket.b {
-      WFWellMarshalledBucketMapI(kbucket, 0);
-      assert kbucket.keys == [key] by {
-        reveal_Image();
-        reveal_B();
-      }
-      assert kbucket == SingletonBucket(key, bucket.b[key]);
-      WeightBucketSingleton(key, kbucket.b[key]);
-    } else {
-      WeightBucketEmpty();
-      WellMarshalledKeyMultiset(kbucket);
-    }
-  }
-
-  lemma WeightBucketInduct(bucket: Bucket, key: Key, msg: Message)
-    requires PreWFBucket(bucket)
-    requires BucketWellMarshalled(bucket)
-    requires key !in bucket.b
-    ensures WeightBucket(B(bucket.b[key := msg])) == WeightBucket(bucket) + WeightKey(key) + WeightMessage(msg)
-  {
-    var newbucket := B(bucket.b[key := msg]);
-    calc {
-      WeightBucket(newbucket);
-      { KeyContribution(newbucket, key); }
-      WeightBucket(Image(newbucket, ExcludeKey(key))) + WeightOneKey(newbucket, key);
-      WeightBucket(Image(newbucket, ExcludeKey(key))) + WeightKey(key) + WeightMessage(msg);
-      {
-        ImageIdentity(bucket, ExcludeKey(key));
-        ImageEquiv(bucket, newbucket, ExcludeKey(key));
-      }
-      WeightBucket(bucket) + WeightKey(key) + WeightMessage(msg);
-    }
-  }
-
-  function ILeftKeys(pivot: Key) : iset<Key> { iset k | Lexicographic_Byte_Order.lt(k, pivot) }
-  function IRightKeys(pivot: Key) : iset<Key> { iset k | Lexicographic_Byte_Order.lte(pivot, k) }
-
-  // used internally
-  lemma SplitBucketImage(bucket: Bucket, pivot: Key)
-    requires WFBucket(bucket)
-    requires BucketWellMarshalled(bucket)
-    ensures SplitBucketLeft(bucket, pivot) == Image(bucket, ILeftKeys(pivot))
-    ensures SplitBucketRight(bucket, pivot) == Image(bucket, IRightKeys(pivot))
-  {
-    reveal_SplitBucketLeft();
-    reveal_SplitBucketRight();
-    reveal_Image();
-    //ImageShape(bucket, ILeftKeys(pivot));
-    //ImageShape(bucket, IRightKeys(pivot));
-  }
-
-  // used internally
-  lemma WMWeightSplitBucketLeft(bucket: Bucket, pivot: Key)
-    requires WFBucket(bucket)
-    requires BucketWellMarshalled(bucket)
-    ensures WeightBucket(SplitBucketLeft(bucket, pivot)) <= WeightBucket(bucket)
-  {
-    SplitBucketImage(bucket, pivot);
-    WeightBucketLinearInKeySet(bucket, ILeftKeys(pivot), AllKeys() - ILeftKeys(pivot));
-  }
 
   lemma WeightSplitBucketLeft(bucket: Bucket, pivot: Key)
     requires WFBucket(bucket)
     //requires BucketWellMarshalled(bucket)
     ensures WeightBucket(SplitBucketLeft(bucket, pivot)) <= WeightBucket(bucket)
   {
-    var wmbucket := Image(bucket, AllKeys());
-    ImageMapIdentity(bucket, AllKeys());
-    WeightWellMarshalledLe(bucket, wmbucket);
-    WMWeightSplitBucketLeft(wmbucket, pivot);
+    var i := BoundedKeyspace.binarySearchIndexOfFirstKeyGte(bucket.keys, pivot);
+    WeightKeyListAdditive(bucket.keys[..i], bucket.keys[i..]);
+    WeightMessageListAdditive(bucket.msgs[..i], bucket.msgs[i..]);
+    assert bucket.keys[..i] + bucket.keys[i..] == bucket.keys;
+    assert bucket.msgs[..i] + bucket.msgs[i..] == bucket.msgs;
     reveal_SplitBucketLeft();
   }
 
   // used internally
-  lemma WMWeightSplitBucketRight(bucket: Bucket, pivot: Key)
-    requires WFBucket(bucket)
-    requires BucketWellMarshalled(bucket)
-    ensures WeightBucket(SplitBucketRight(bucket, pivot)) <= WeightBucket(bucket)
-  {
-    SplitBucketImage(bucket, pivot);
-    WeightBucketLinearInKeySet(bucket, AllKeys() - IRightKeys(pivot), IRightKeys(pivot));
-  }
 
   lemma WeightSplitBucketRight(bucket: Bucket, pivot: Key)
     requires WFBucket(bucket)
     //requires BucketWellMarshalled(bucket)
     ensures WeightBucket(SplitBucketRight(bucket, pivot)) <= WeightBucket(bucket)
   {
-    var wmbucket := Image(bucket, AllKeys());
-    ImageMapIdentity(bucket, AllKeys());
-    WeightWellMarshalledLe(bucket, wmbucket);
-    WMWeightSplitBucketRight(wmbucket, pivot);
+    var i := BoundedKeyspace.binarySearchIndexOfFirstKeyGte(bucket.keys, pivot);
+    WeightKeyListAdditive(bucket.keys[..i], bucket.keys[i..]);
+    WeightMessageListAdditive(bucket.msgs[..i], bucket.msgs[i..]);
+    assert bucket.keys[..i] + bucket.keys[i..] == bucket.keys;
+    assert bucket.msgs[..i] + bucket.msgs[i..] == bucket.msgs;
     reveal_SplitBucketRight();
   }
 
   lemma WeightSplitBucketAdditive(bucket: Bucket, pivot: Key)
-    requires WFBucket(bucket)
-    requires BucketWellMarshalled(bucket)
+    requires PreWFBucket(bucket)
     ensures WeightBucket(SplitBucketLeft(bucket, pivot)) +
             WeightBucket(SplitBucketRight(bucket, pivot)) == WeightBucket(bucket)
   {
-    SplitBucketImage(bucket, pivot);
-    WeightBucketLinearInKeySet(bucket, ILeftKeys(pivot), IRightKeys(pivot));
-  }
-
-  lemma WeightSplitBucketAdditiveLe(bucket: Bucket, pivot: Key)
-    requires WFBucket(bucket)
-    //requires BucketWellMarshalled(bucket)
-    ensures WeightBucket(SplitBucketLeft(bucket, pivot)) +
-            WeightBucket(SplitBucketRight(bucket, pivot)) <= WeightBucket(bucket)
-  {
-    var wmbucket := Image(bucket, AllKeys());
-    ImageMapIdentity(bucket, AllKeys());
-    WeightWellMarshalledLe(bucket, wmbucket);
-    reveal_SplitBucketLeft();
-    reveal_SplitBucketRight();
-    WeightSplitBucketAdditive(wmbucket, pivot);
+    var l := SplitBucketLeft(bucket, pivot);
+    var r := SplitBucketRight(bucket, pivot);
+    assert bucket.keys == l.keys + r.keys
+        && bucket.msgs == l.msgs + r.msgs 
+    by {
+      reveal_SplitBucketLeft();
+      reveal_SplitBucketRight();
+    }
+    WeightKeyListAdditive(l.keys, r.keys);
+    WeightMessageListAdditive(l.msgs, r.msgs);
   }
 
   lemma WeightBucketList2(a: Bucket, b: Bucket)
@@ -755,13 +414,6 @@ module BucketWeights {
         WeightBucketList(left) + WeightBucketList(right);
       }
     }
-  }
-
-  lemma WeightBucketListConcatOne(left: BucketList, extra: Bucket)
-    ensures WeightBucketList(left + [extra]) == WeightBucketList(left) + WeightBucket(extra)
-  {
-    WeightBucketListConcat(left, [extra]);
-    reveal_WeightBucketList();
   }
 
   lemma WeightBucketListSlice(blist: BucketList, a: int, b: int)
@@ -837,337 +489,6 @@ module BucketWeights {
     }
   }
 
-  function RouteRange(pivots: PivotTable, i: int) : iset<Key>
-    requires WFPivots(pivots)
-  {
-    iset k | BoundedKey(pivots, k) && Route(pivots, k) == i
-  }
-
-  // used internally
-  lemma WeightBucketListItemFlushSingletonOrEmpty(parent: Bucket, children: BucketList, pivots: PivotTable, i: int, filter:iset<Key>, key:Key)
-    requires WFPivots(pivots)
-    requires WFBucket(parent)
-    requires BucketWellMarshalled(parent)
-    requires 0 <= i < |children|
-    requires WFBucket(children[i])
-    requires BucketListWellMarshalled(children)
-    requires forall k :: k in filter ==> k == key   // filter admits at most one key
-    ensures WeightBucket(BucketListItemFlush(Image(parent, filter), Image(children[i], filter), pivots, i))
-    <= WeightBucket(Image(parent, RouteRange(pivots, i) * filter))
-    + WeightBucket(Image(children[i], RouteRange(pivots, i) * filter));
-  {
-    reveal_Image();
-
-    var flush := BucketListItemFlush(Image(parent, filter), Image(children[i], filter), pivots, i);
-    if key in flush.b.Keys {
-      WellMarshalledBucketsEq(flush, SingletonBucket(key, flush.b[key]));
-      WeightBucketSingleton(key, flush.b[key]);
-    } else {
-      WellMarshalledBucketsEq(flush, EmptyBucket());
-      WeightBucketEmpty();
-    }
-
-    var filteredParent := Image(parent, RouteRange(pivots, i) * filter);
-    if key in filteredParent.b {
-      WellMarshalledBucketsEq(filteredParent, SingletonBucket(key, filteredParent.b[key]));
-      WeightBucketSingleton(key, filteredParent.b[key]);
-    } else {
-      WellMarshalledBucketsEq(filteredParent, EmptyBucket());
-      WeightBucketEmpty();
-    }
-
-    var filteredChild := Image(children[i], RouteRange(pivots, i) * filter);
-    if key in filteredChild.b {
-      WellMarshalledBucketsEq(filteredChild, SingletonBucket(key, filteredChild.b[key]));
-      WeightBucketSingleton(key, filteredChild.b[key]);
-    } else {
-      WellMarshalledBucketsEq(filteredChild, EmptyBucket());
-      WeightBucketEmpty();
-    }
-
-    if (key in filteredChild.b && key in filteredParent.b && key in flush.b) {
-      // This is the only tricksy case, where we actually care how Merge
-      // affects weights of the messages getting swapped.
-      MergeGainsNoWeight(BucketGet(filteredParent, key), BucketGet(filteredChild, key));
-    }
-  }
-
-  // used internally
-  lemma WeightBucketFilterPartitions(bucket:Bucket, filter:iset<Key>, a:iset<Key>, b:iset<Key>)
-    requires WFBucket(bucket)
-    requires BucketWellMarshalled(bucket)
-    requires a !! b
-    requires filter * a + filter * b == filter;
-    ensures WeightBucket(Image(bucket, filter)) ==
-      WeightBucket(Image(bucket, filter * a)) + WeightBucket(Image(bucket, filter * b));
-  {
-    calc {
-      WeightBucket(Image(bucket, filter));
-        {
-          ImageShape(bucket, filter);
-          WeightBucketLinearInKeySet(Image(bucket, filter), a, b);
-        }
-      WeightBucket(Image(Image(bucket, filter), a)) + WeightBucket(Image(Image(bucket, filter), b));
-        {
-          ImageIntersect(bucket, filter, a);
-          ImageIntersect(bucket, filter, b);
-        }
-      WeightBucket(Image(bucket, filter * a)) + WeightBucket(Image(bucket, filter * b));
-    }
-  }
-
-  // used internally
-  lemma WeightBucketListItemFlushInner(parent: Bucket, children: BucketList, pivots: PivotTable, i: int, filter:iset<Key>)
-    requires WFBucket(parent)
-    requires BucketWellMarshalled(parent)
-    requires forall i | 0 <= i < |children| :: WFBucket(children[i])
-    requires BucketListWellMarshalled(children)
-    requires WFPivots(pivots)
-    requires 0 <= i < |children|
-    ensures
-    WeightBucket(BucketListItemFlush(Image(parent, filter), Image(children[i], filter), pivots, i))
-    <= WeightBucket(Image(parent, RouteRange(pivots, i) * filter)) + WeightBucket(Image(children[i], RouteRange(pivots, i) * filter))
-  decreases |Image(parent, filter).b| + |Image(children[i], filter).b|
-  {
-    // Pick an arbitrary key to decrease by
-    // (In Lisp, "car" is the first thing in a list, "cdr" is everything else.)
-    var carKey;
-    if |Image(parent, filter).b| != 0 {
-      carKey :| carKey in Image(parent, filter).b;
-    } else if |Image(children[i], filter).b| != 0 {
-      carKey :| carKey in Image(children[i], filter).b;
-    } else {
-      WellMarshalledBucketsEq(BucketListItemFlush(Image(parent, filter), Image(children[i], filter), pivots, i), EmptyBucket());
-      WeightBucketEmpty();
-      return;
-    }
-
-    var carFilter := IncludeKey(carKey);
-    var cdrFilter := ExcludeKey(carKey);
-
-    // cdrFilter decreases
-    if |Image(parent, filter).b| != 0 {
-      forall ensures |Image(parent, filter * cdrFilter).b| < |Image(parent, filter).b|
-      {
-        reveal_Image();
-        Sets.ProperSubsetImpliesSmallerCardinality(Image(parent, filter * cdrFilter).b.Keys, Image(parent, filter).b.Keys);
-      }
-      ImageSubset(children[i], filter * cdrFilter, filter);
-      Sets.SetInclusionImpliesSmallerCardinality(Image(children[i], filter * cdrFilter).b.Keys, Image(children[i], filter).b.Keys);
-    } else {
-      ImageSubset(parent, filter * cdrFilter, filter);
-      Sets.SetInclusionImpliesSmallerCardinality(Image(parent, filter * cdrFilter).b.Keys, Image(parent, filter).b.Keys);
-      forall ensures |Image(children[i], filter * cdrFilter).b| < |Image(children[i], filter).b|
-      {
-        reveal_Image();
-        Sets.ProperSubsetImpliesSmallerCardinality(Image(children[i], filter * cdrFilter).b.Keys, Image(children[i], filter).b.Keys);
-      }
-    }
-
-    // The core of the proof is that the inequality holds for the carKey we chose from the parent.
-    forall k | k in BucketListItemFlush(Image(parent, filter * carFilter), Image(children[i], filter * carFilter), pivots, i).b.Keys
-      ensures k == carKey
-    {
-      reveal_Image();
-    }
-
-    calc {
-      WeightBucket(BucketListItemFlush(Image(parent, filter), Image(children[i], filter), pivots, i));
-        {
-          WeightBucketLinearInKeySet(
-            BucketListItemFlush(Image(parent, filter), Image(children[i], filter), pivots, i), carFilter, cdrFilter);
-        }
-      WeightBucket(Image(BucketListItemFlush(Image(parent, filter), Image(children[i], filter), pivots, i), carFilter))
-      + WeightBucket(Image(BucketListItemFlush(Image(parent, filter), Image(children[i], filter), pivots, i), cdrFilter));
-        { // push filters through Image operator & BucketListItemFlush.
-          reveal_Image();
-          WellMarshalledBucketsEq(
-            Image(BucketListItemFlush(Image(parent, filter), Image(children[i], filter), pivots, i), carFilter),
-            BucketListItemFlush(Image(parent, filter * carFilter), Image(children[i], filter * carFilter), pivots, i)
-          );
-          WellMarshalledBucketsEq(
-            Image(BucketListItemFlush(Image(parent, filter), Image(children[i], filter), pivots, i), cdrFilter),
-            BucketListItemFlush(Image(parent, filter * cdrFilter), Image(children[i], filter * cdrFilter), pivots, i)
-          );
-        }
-      WeightBucket(BucketListItemFlush(Image(parent, filter * carFilter), Image(children[i], filter * carFilter), pivots, i))
-      + WeightBucket(BucketListItemFlush(Image(parent, filter * cdrFilter), Image(children[i], filter * cdrFilter), pivots, i));
-      <=
-        { // recursion for car
-          WeightBucketListItemFlushSingletonOrEmpty(parent, children, pivots, i, filter * carFilter, carKey);
-          assert RouteRange(pivots, i) * (filter * carFilter) == RouteRange(pivots, i) * filter * carFilter;
-          // recursion for cdr
-          WeightBucketListItemFlushInner(parent, children, pivots, i, filter * cdrFilter);
-          assert RouteRange(pivots, i) * (filter * cdrFilter) == RouteRange(pivots, i) * filter * cdrFilter;
-        }
-      WeightBucket(Image(parent, RouteRange(pivots, i) * filter * carFilter)) + WeightBucket(Image(children[i], RouteRange(pivots, i) * filter * carFilter))
-        + WeightBucket(Image(parent, RouteRange(pivots, i) * filter * cdrFilter)) + WeightBucket(Image(children[i], RouteRange(pivots, i) * filter * cdrFilter));
-      // Just rearranging terms
-      WeightBucket(Image(parent, RouteRange(pivots, i) * filter * carFilter))
-        + WeightBucket(Image(parent, RouteRange(pivots, i) * filter * cdrFilter))
-        + WeightBucket(Image(children[i], RouteRange(pivots, i) * filter * carFilter))
-        + WeightBucket(Image(children[i], RouteRange(pivots, i) * filter * cdrFilter));
-      { WeightBucketFilterPartitions(parent, RouteRange(pivots, i) * filter, carFilter, cdrFilter); }
-      WeightBucket(Image(parent, RouteRange(pivots, i) * filter))
-        + WeightBucket(Image(children[i], RouteRange(pivots, i) * filter * carFilter))
-        + WeightBucket(Image(children[i], RouteRange(pivots, i) * filter * cdrFilter));
-      { WeightBucketFilterPartitions(children[i], RouteRange(pivots, i) * filter, carFilter, cdrFilter); }
-      WeightBucket(Image(parent, RouteRange(pivots, i) * filter))
-        + WeightBucket(Image(children[i], RouteRange(pivots, i) * filter));
-    }
-  }
-
-  // used internally
-  lemma WeightBucketListItemFlush(parent: Bucket, children: BucketList, pivots: PivotTable, i: int)
-  requires WFPivots(pivots)
-  requires 0 <= i < |children|
-  requires WFBucket(parent)
-  requires BucketWellMarshalled(parent)
-  requires forall i | 0 <= i < |children| :: WFBucket(children[i])
-  requires BucketListWellMarshalled(children)
-  ensures WeightBucket(BucketListItemFlush(parent, children[i], pivots, i))
-      <= WeightBucket(Image(parent, RouteRange(pivots, i))) + WeightBucket(Image(children[i], RouteRange(pivots, i)))
-  {
-    WeightBucketListItemFlushInner(parent, children, pivots, i, AllKeys());
-    ImageIdentity(parent, AllKeys());
-    ImageIdentity(children[i], AllKeys());
-    reveal_Image();
-    assert Image(parent, RouteRange(pivots, i) * AllKeys()) == Image(parent, RouteRange(pivots, i));  // trigger
-    assert Image(children[i], RouteRange(pivots, i) * AllKeys()) == Image(children[i], RouteRange(pivots, i));  // trigger
-  }
-
-  function RouteRanges(pivots: PivotTable, i: int) : iset<Key>
-    // Keys that route to children < i
-    requires WFPivots(pivots)
-  {
-    iset k | BoundedKey(pivots, k) && Route(pivots, k) < i
-  }
-
-  // The sequence axioms were responsible for creating a timeout in the rich
-  // context where this was used; hence this ugly workaround.
-  lemma SequenceSingleton<T>(s:seq<T>, i:int)
-  requires 0 <= i < |s|
-  ensures s[i..i+1] == [s[i]];
-  {
-  }
-
-  // used internally
-  lemma WMWeightBucketListFlushPartial(parent: Bucket, children: BucketList, pivots: PivotTable, items: int)
-  requires WFBucketListProper(children, pivots)
-  requires 0 <= items <= |children|
-  requires WFBucket(parent)
-  requires BucketWellMarshalled(parent)
-  requires BucketListWellMarshalled(children)
-  ensures WeightBucketList(BucketListFlushPartial(parent, children, pivots, items))
-      <= WeightBucket(Image(parent, RouteRanges(pivots, items)))
-        + WeightBucketList(children[..items])
-  {
-    if items == 0 {
-    } else {
-      calc {
-        WeightBucketList(BucketListFlushPartial(parent, children, pivots, items));
-          { // Break off the last element as a sublist.
-            WeightBucketListConcat(BucketListFlushPartial(parent, children, pivots, items - 1),
-              [BucketListItemFlush(parent, children[items - 1], pivots, items - 1)]);
-          }
-        WeightBucketList(BucketListFlushPartial(parent, children, pivots, items - 1))
-          + WeightBucketList([BucketListItemFlush(parent, children[items - 1], pivots, items - 1)]);
-          { reveal_WeightBucketList(); }  // from singleton list to bucket
-        WeightBucketList(BucketListFlushPartial(parent, children, pivots, items - 1))
-          + WeightBucket(BucketListItemFlush(parent, children[items - 1], pivots, items - 1));
-        <=
-          { WMWeightBucketListFlushPartial(parent, children, pivots, items - 1); }  // Recurse on prefix
-        WeightBucket(Image(parent, RouteRanges(pivots, items - 1)))
-          + WeightBucketList(children[..items - 1])
-          + WeightBucket(BucketListItemFlush(parent, children[items - 1], pivots, items - 1));
-        <=
-          { WeightBucketListItemFlush(parent, children, pivots, items -1); }  // Flush the singleton
-        WeightBucket(Image(parent, RouteRanges(pivots, items - 1)))
-          + WeightBucketList(children[..items - 1])
-          + WeightBucket(Image(parent, RouteRange(pivots, items - 1)))
-          + WeightBucket(Image(children[items - 1], RouteRange(pivots, items - 1)));
-        {  // Glue the parent halves back together
-          WeightBucketLinearInKeySetSum(parent, RouteRanges(pivots, items - 1), RouteRange(pivots, items - 1));
-          assert RouteRanges(pivots, items) == RouteRanges(pivots, items - 1) + RouteRange(pivots, items - 1);  // trigger
-        }
-        WeightBucket(Image(parent, RouteRanges(pivots, items)))
-          + WeightBucketList(children[..items - 1])
-          + WeightBucket(Image(children[items - 1], RouteRange(pivots, items - 1)));
-        { // The last child bucket's RouteRange covers the whole bucket, so we can simplify.
-          ImageShape(children[items - 1], RouteRange(pivots, items - 1));
-          WellMarshalledBucketsEq(Image(children[items - 1], RouteRange(pivots, items - 1)), children[items-1]);
-        }
-        WeightBucket(Image(parent, RouteRanges(pivots, items)))
-          + WeightBucketList(children[..items-1]) + WeightBucket(children[items-1]);
-        { // pack the last bucket up into a singleton list
-          SequenceSingleton(children, items-1);
-          //assert children[items-1..items] == [children[items-1]]; // trigger
-          reveal_WeightBucketList();
-        }
-        WeightBucket(Image(parent, RouteRanges(pivots, items)))
-          + WeightBucketList(children[..items-1]) + WeightBucket(children[items-1]);
-        { // and glue the children sublists back together
-          WeightBucketListConcatOne(children[..items-1], children[items-1]);
-          assert children[..items-1] + [children[items-1]] == children[..items]; // trigger
-        }
-        WeightBucket(Image(parent, RouteRanges(pivots, items)))
-          + WeightBucketList(children[..items]);
-      }
-    }
-  }
-
-  // used internally
-  lemma WMWeightBucketListFlush(parent: Bucket, children: BucketList, pivots: PivotTable)
-  requires WFBucketListProper(children, pivots)
-  requires |children| == NumBuckets(pivots)
-  requires WFBucket(parent)
-  requires BucketWellMarshalled(parent)
-  requires forall key | key in parent.b.Keys :: BoundedKey(pivots, key)
-  // requires forall i | 0 <= i < |children| :: WFBucket(children[i])
-  requires BucketListWellMarshalled(children)
-  ensures WeightBucketList(BucketListFlush(parent, children, pivots))
-      <= WeightBucket(parent) + WeightBucketList(children)
-  {
-    WMWeightBucketListFlushPartial(parent, children, pivots, |children|);
-    forall ensures Image(parent, RouteRanges(pivots, |children|)) == parent
-    {
-      reveal_Image();
-      WellMarshalledBucketsEq(Image(parent, RouteRanges(pivots, |children|)), parent);
-    }
-    assert children[..|children|] == children;  // trigger
-  }
-
-  // used
-  lemma WeightBucketListFlush(parent: Bucket, children: BucketList, pivots: PivotTable)
-  requires WFBucketList(children, pivots)
-  requires |children| == NumBuckets(pivots)
-  requires WFBucket(parent)
-  requires forall key | key in parent.b.Keys :: BoundedKey(pivots, key)
-  //requires forall i | 0 <= i < |children| :: WFBucket(children[i])
-  //requires BucketListWellMarshalled(children)
-  ensures WeightBucketList(BucketListFlush(parent, children, pivots))
-      <= WeightBucket(parent) + WeightBucketList(children)
-  {
-    var wmparent := Image(parent, AllKeys());
-    var cchildren := seq(|children|, i requires 0 <= i < |children| => ClampToSlot(children[i], pivots, i));
-    
-    ImageMapIdentity(parent, AllKeys());
-    forall i: nat | i < |children|
-      ensures ClampToSlot(children[i], pivots, i) == ClampToSlot(cchildren[i], pivots, i)
-      ensures WeightBucket(cchildren[i]) <= WeightBucket(children[i])
-    {
-      var c := ClampToSlot(children[i], pivots, i);
-      var cc := ClampToSlot(cchildren[i], pivots, i);
-      WellMarshalledBucketsEq(c, cc);
-      WeightWellMarshalledSubsetLe(cchildren[i], children[i]);
-    }
-
-    WeightWellMarshalledLe(parent, wmparent);
-    WeightWellMarshalledListPointwiseLe(children, cchildren);
-    WMWeightBucketListFlush(wmparent, cchildren, pivots);
-    BucketListFlushPartialDependsOnlyOnB(wmparent, cchildren, parent, children, pivots, |cchildren|);
-  }
-  
   // used internally
   lemma WeightBucketListReplace(blist: BucketList, i: int, bucket: Bucket)
   requires 0 <= i < |blist|
@@ -1204,20 +525,11 @@ module BucketWeights {
     WeightBucketListReplace(blist, i, bucket);
   }
 
-  // used
-  lemma WeightBucketListClearEntry(blist: BucketList, i: int)
-  requires 0 <= i < |blist|
-  ensures WeightBucketList(blist[i := B(map[])]) <= WeightBucketList(blist)
-  {
-    WeightBucketListReplace(blist, i, B(map[]));
-  }
-
   // Analogous to WeightBucketListReplace, except we're changing the size of the subsequence in the middle.
   // used internally
   lemma WeightSplitBucketInList(blist: BucketList, i: int, pivot: Key)
     requires 0 <= i < |blist|
     requires WFBucket(blist[i])
-    requires BucketWellMarshalled(blist[i])
     ensures WeightBucketList(SplitBucketInList(blist, i, pivot))
     == WeightBucketList(blist)
   {
@@ -1257,49 +569,6 @@ module BucketWeights {
   }
 
   // used
-  lemma WeightSplitBucketInListLe(blist: BucketList, i: int, pivot: Key)
-   requires 0 <= i < |blist|
-   requires WFBucket(blist[i])
-   ensures WeightBucketList(SplitBucketInList(blist, i, pivot))
-           <= WeightBucketList(blist)
-  {
-    var newblist := blist[i := B(blist[i].b)];
-    calc <= {
-      WeightBucketList(SplitBucketInList(blist, i, pivot));
-      {
-        reveal_SplitBucketInList();
-        reveal_SplitBucketRight();
-        reveal_SplitBucketLeft();
-        reveal_replace1with2();
-        assert blist[..i] == newblist[..i];
-        assert blist[i+1..] == newblist[i+1..];
-      }
-      WeightBucketList(SplitBucketInList(newblist, i, pivot));
-      { WeightSplitBucketInList(newblist, i, pivot); }
-      WeightBucketList(newblist);
-      {
-        assert newblist == newblist[..i] + newblist[i..];
-        assert newblist[i..] == newblist[i..i+1] + newblist[i+1..];
-        WeightBucketListConcat(newblist[..i], newblist[i..]);
-        WeightBucketListConcat(newblist[i..i+1], newblist[i+1..]);
-      }
-      WeightBucketList(newblist[..i]) + WeightBucketList(newblist[i..i+1]) + WeightBucketList(newblist[i+1..]);
-      {
-        WeightWellMarshalledLe(blist[i], newblist[i]);
-        reveal_WeightBucketList();
-      }
-      WeightBucketList(newblist[..i]) + WeightBucketList(blist[i..i+1]) + WeightBucketList(newblist[i+1..]);
-      {
-        assert blist == blist[..i] + blist[i..];
-        assert blist[i..] == blist[i..i+1] + blist[i+1..];
-        WeightBucketListConcat(blist[..i], blist[i..]);
-        WeightBucketListConcat(blist[i..i+1], blist[i+1..]);
-      }
-      WeightBucketList(blist);
-    }
-  }
-
-  // used
   lemma WeightBucketListSuffix(blist: BucketList, a: int)
   requires 0 <= a <= |blist|
   ensures WeightBucketList(blist[a..]) <= WeightBucketList(blist)
@@ -1308,275 +577,6 @@ module BucketWeights {
     assert blist == blist[..a] + blist[a..];
   }
 
-  // used internally
-  lemma MergedKeyMultisets(left: Bucket, right: Bucket)
-    requires PreWFBucket(left)
-    requires PreWFBucket(right)
-    ensures multiset(MergeBuckets(left, right).keys) <= multiset(left.keys) + multiset(right.keys)
-  {
-    var merged := MergeBuckets(left, right);
-    var fn := Multisets.ValueMultisetFn(merged.b);
-    calc <= {
-      multiset(merged.keys);
-      { WellMarshalledKeyMultiset(merged); }
-      multiset(merged.b.Keys);
-      { reveal_MergeBuckets(); }
-      //multiset(left.b.Keys) + multiset(right.b.Keys);
-      multiset(left.keys) + multiset(right.keys);
-    }
-  }
-
-  // used internally
-  lemma MergedMessageMultisets(left: Bucket, right: Bucket)
-    requires PreWFBucket(left)
-    requires PreWFBucket(right)
-    ensures multiset(MergeBuckets(left, right).msgs) <= multiset(left.msgs) + multiset(right.msgs)
-  {
-    var merged := MergeBuckets(left, right);
-    var fn := Multisets.ValueMultisetFn(merged.b);
-    calc <= {
-      multiset(merged.msgs);
-      { WFMessageMultiset(merged); }
-      Multisets.ValueMultiset(merged.b);
-      Multisets.Apply(fn, multiset(merged.b.Keys));
-      {
-        reveal_MergeBuckets();
-        Multisets.ApplyMonotonic(fn,
-                                 multiset(merged.b.Keys),
-                                 multiset(left.b.Keys) + (multiset(right.b.Keys) - multiset(left.b.Keys)));
-      }
-      Multisets.Apply(fn, multiset(left.b.Keys) + (multiset(right.b.Keys) - multiset(left.b.Keys)));
-      {
-        Multisets.ApplyAdditive(fn, multiset(left.b.Keys), (multiset(right.b.Keys) - multiset(left.b.Keys)));
-      }
-      Multisets.Apply(fn, multiset(left.b.Keys))
-        + Multisets.Apply(fn, (multiset(right.b.Keys) - multiset(left.b.Keys)));
-      {
-        reveal_MergeBuckets();
-        Multisets.ApplyEquivalentFns(fn, Multisets.ValueMultisetFn(left.b), multiset(left.b.Keys));
-      }
-      Multisets.Apply(Multisets.ValueMultisetFn(left.b), multiset(left.b.Keys))
-        + Multisets.Apply(fn, (multiset(right.b.Keys) - multiset(left.b.Keys)));
-      {
-      }
-      Multisets.Apply(Multisets.ValueMultisetFn(left.b), multiset(left.b.Keys))
-        + Multisets.Apply(fn, (multiset(right.b.Keys) - multiset(left.b.Keys)));
-      Multisets.ValueMultiset(left.b)
-        + Multisets.Apply(fn, (multiset(right.b.Keys) - multiset(left.b.Keys)));
-      {
-        reveal_MergeBuckets();
-        Multisets.ApplyEquivalentFns(fn, Multisets.ValueMultisetFn(right.b),
-                                     multiset(right.b.Keys) - multiset(left.b.Keys));
-      }
-      Multisets.ValueMultiset(left.b)
-        + Multisets.Apply(Multisets.ValueMultisetFn(right.b), multiset(right.b.Keys) - multiset(left.b.Keys));
-      {
-        Multisets.ApplyMonotonic(Multisets.ValueMultisetFn(right.b),
-                                 multiset(right.b.Keys) - multiset(left.b.Keys),
-                                 multiset(right.b.Keys));
-      }
-      Multisets.ValueMultiset(left.b) + Multisets.ValueMultiset(right.b);
-      {
-        WFMessageMultiset(left);
-        WFMessageMultiset(right);
-      }
-      multiset(left.msgs) + multiset(right.msgs);
-    }
-  }    
-
-  // used
-  lemma WeightMergeBuckets(left: Bucket, right: Bucket)
-    requires PreWFBucket(left)
-    requires PreWFBucket(right)
-    ensures WeightBucket(MergeBuckets(left, right)) <= WeightBucket(left) + WeightBucket(right)
-  {
-    var merged := MergeBuckets(left, right);
-    MergedKeyMultisets(left, right);
-    MergedMessageMultisets(left, right);
-
-    calc <= {
-      WeightKeyMultiset(multiset(merged.keys));
-      {
-        assert multiset(left.keys) + multiset(right.keys) ==
-          multiset(merged.keys) + ((multiset(left.keys) + multiset(right.keys)) - multiset(merged.keys));
-        WeightKeyMultisetAdditive(multiset(merged.keys),
-                                  (multiset(left.keys) + multiset(right.keys)) - multiset(merged.keys));
-      }
-      WeightKeyMultiset(multiset(left.keys) + multiset(right.keys));
-      { WeightKeyMultisetAdditive(multiset(left.keys), multiset(right.keys)); }
-      WeightKeyMultiset(multiset(left.keys)) + WeightKeyMultiset(multiset(right.keys));
-    }
-    
-    calc <= {
-      WeightMessageMultiset(multiset(merged.msgs));
-      {
-        assert multiset(left.msgs) + multiset(right.msgs) ==
-          multiset(merged.msgs) + ((multiset(left.msgs) + multiset(right.msgs)) - multiset(merged.msgs));
-        WeightMessageMultisetAdditive(multiset(merged.msgs),
-                                     (multiset(left.msgs) + multiset(right.msgs)) - multiset(merged.msgs));
-      }
-      WeightMessageMultiset(multiset(left.msgs) + multiset(right.msgs));
-      { WeightMessageMultisetAdditive(multiset(left.msgs), multiset(right.msgs)); }
-      WeightMessageMultiset(multiset(left.msgs)) + WeightMessageMultiset(multiset(right.msgs));
-    }
-  }
-
-  // used
-  lemma WeightMergeBucketsInListLe(blist: BucketList, i: int, pivots: PivotTable)
-  requires 0 <= i < |blist| - 1
-  requires PreWFBucket(blist[i])
-  requires PreWFBucket(blist[i+1])
-  ensures WeightBucketList(MergeBucketsInList(blist, i)) <= WeightBucketList(blist)
-  {
-    var newblist := MergeBucketsInList(blist, i);
-    calc <= {
-      WeightBucketList(newblist);
-      {
-        assert newblist == newblist[..i] + newblist[i..];
-        assert newblist[i..] == newblist[i..i+1] + newblist[i+1..];
-        WeightBucketListConcat(newblist[..i], newblist[i..]);
-        WeightBucketListConcat(newblist[i..i+1], newblist[i+1..]);
-      }
-      WeightBucketList(newblist[..i]) + WeightBucketList(newblist[i..i+1]) + WeightBucketList(newblist[i+1..]);
-      { reveal_WeightBucketList(); }
-      WeightBucketList(newblist[..i]) + WeightBucket(newblist[i]) + WeightBucketList(newblist[i+1..]);
-      {
-        reveal_MergeBucketsInList();
-        WeightMergeBuckets(blist[i], blist[i+1]);
-      }
-      WeightBucketList(newblist[..i]) + WeightBucket(blist[i]) + WeightBucket(blist[i+1]) + WeightBucketList(newblist[i+1..]);
-      { reveal_WeightBucketList(); }
-      WeightBucketList(newblist[..i]) + WeightBucketList(blist[i..i+2]) + WeightBucketList(newblist[i+1..]);
-      {
-        reveal_MergeBucketsInList();
-        assert blist[..i] == newblist[..i];
-        assert blist[i+2..] == newblist[i+1..];
-      }
-      WeightBucketList(blist[..i]) + WeightBucketList(blist[i..i+2]) + WeightBucketList(blist[i+2..]);
-      {
-        assert blist == blist[..i] + blist[i..];
-        assert blist[i..] == blist[i..i+2] + blist[i+2..];
-        WeightBucketListConcat(blist[..i], blist[i..]);
-        WeightBucketListConcat(blist[i..i+2], blist[i+2..]);
-      }
-      WeightBucketList(blist);
-    }
-  }
-
-  // used internally
-  lemma WeightBucketSubset(bucket:Bucket, a:iset<Key>, b:iset<Key>)
-    requires a<=b
-    ensures WeightBucket(Image(bucket, a)) <= WeightBucket(Image(bucket, b))
-  {
-    calc {
-      WeightBucket(Image(bucket, a));
-        { ImageSubset(bucket, a, b); }
-      WeightBucket(Image(Image(bucket, b), a));
-      <=
-      WeightBucket(Image(Image(bucket, b), a)) + WeightBucket(Image(Image(bucket, b), b-a));
-        {
-          ImageShape(bucket, b);
-          WeightBucketLinearInKeySet(Image(bucket, b), a, b-a);
-        }
-      WeightBucket(Image(bucket, b));
-    }
-  }
-
-  // TODO(thance): Why do we have both MergeBuckets and JoinBucketList? The
-  // former is nice because it obeys the WFBucketList discipline, and can hence
-  // draw tight conclusions (WeightBucketList == WeightBucketList). Can we
-  // redefine JoinBucketList in terms of MergBuckets and lose some cruft?
-  // used
-  lemma WeightJoinBucketList(blist: BucketList)
-    requires forall i | 0 <= i < |blist| :: PreWFBucket(blist[i])
-    ensures WeightBucket(JoinBucketList(blist)) <= WeightBucketList(blist)
-  {
-    if |blist| == 0 {
-    } else {
-      calc <= {
-        WeightBucket(JoinBucketList(blist));
-        //WeightBucket(B(MapUnion(JoinBucketList(DropLast(blist)).b, Last(blist).b)));
-        {
-          reveal_MergeBuckets();
-          reveal_MapUnion();
-          WeightMergeBuckets(JoinBucketList(DropLast(blist)), Last(blist));
-        }
-        WeightBucket(JoinBucketList(DropLast(blist))) + WeightBucket(Last(blist));
-        //WeightBucketList(DropLast(blist)) + WeightBucket(Last(blist));
-        { reveal_WeightBucketList(); }
-        WeightBucketList(blist);
-      }
-    }
-  }
-
-  // used internaly
-  lemma WMWeightSplitBucketOnPivots(bucket: Bucket, pivots: PivotTable)
-    requires PreWFBucket(bucket)
-    requires BoundedBucket(bucket, pivots)
-    requires BucketWellMarshalled(bucket)
-    ensures WeightBucketList(SplitBucketOnPivots(bucket, pivots)) == WeightBucket(bucket)
-    decreases |pivots|
-  {
-    if |pivots| == 2 {
-      calc {
-        WeightBucketList(SplitBucketOnPivots(bucket, pivots));
-        WeightBucketList([B(bucket.b)]);
-        { reveal_WeightBucketList(); }
-        WeightBucket(B(bucket.b));
-        { WellMarshalledBucketsEq(B(bucket.b), bucket); }
-        WeightBucket(bucket);
-      }
-    } else {
-      var piv := GetKey(pivots, NumBuckets(pivots)-1);
-      var pivots' := remove(pivots, NumBuckets(pivots)-1);
-      WFPivotsRemoved(pivots, NumBuckets(pivots)-1);
-
-      var l := SplitBucketLeft(bucket, piv);
-      var r := SplitBucketRight(bucket, piv);
-      reveal_SplitBucketLeft();
-      reveal_SplitBucketRight();
-
-      var lKeys := iset k | k in l.b;
-      var rKeys := iset k | k in r.b;
-      
-      calc {
-        WeightBucketList(SplitBucketOnPivots(bucket, pivots));  // defn.
-        WeightBucketList(SplitBucketOnPivots(l, pivots') + [r]);  // defn.
-          { WeightBucketListConcatOne(SplitBucketOnPivots(l, pivots'), r); } // break off tail
-        WeightBucketList(SplitBucketOnPivots(l, pivots')) + WeightBucket(r);
-          { WMWeightSplitBucketOnPivots(l, pivots'); }
-        WeightBucket(l) + WeightBucket(r);
-          {
-            ImageTrim(bucket, lKeys, l);
-            ImageTrim(bucket, rKeys, r);
-            WellMarshalledBucketsEq(l, Image(bucket, lKeys));
-            WellMarshalledBucketsEq(r, Image(bucket, rKeys));            
-          }
-        WeightBucket(Image(bucket, lKeys)) + WeightBucket(Image(bucket, rKeys));
-          { WeightBucketLinearInKeySetSum(bucket, lKeys, rKeys); }
-        WeightBucket(Image(bucket, lKeys + rKeys));
-          { ImageIdentity(bucket, lKeys + rKeys); }
-        WeightBucket(bucket);
-      }
-    }
-  }
-
-  lemma WeightSplitBucketOnPivots(bucket: Bucket, pivots: PivotTable)
-    requires PreWFBucket(bucket)
-    requires WFPivots(pivots)
-    requires BoundedBucket(bucket, pivots)
-    ensures WeightBucketList(SplitBucketOnPivots(bucket, pivots)) <= WeightBucket(bucket)
-    decreases |pivots|
-  {
-    var wmbucket := Image(bucket, AllKeys());
-    ImageMapIdentity(bucket, AllKeys());
-    WeightWellMarshalledLe(bucket, wmbucket);
-    WMWeightSplitBucketOnPivots(wmbucket, pivots);
-    reveal_SplitBucketLeft();
-    reveal_SplitBucketRight();
-  }
-  
-  // used (in KVList)
   lemma KeyMultisetLeWeight(keys: multiset<Key>)
     ensures 4 * |keys| <= WeightKeyMultiset(keys)
   {
@@ -1605,14 +605,13 @@ module BucketWeights {
       }
     }
   }
-  
+
   // This is far weaker than it could be, but it's probably good enough.
   // Weight is on the order of a few million, and I plan on using this lemma
   // to show that numbers fit within 64 bits.
   lemma NumElementsLteWeight(bucket: Bucket)
     requires PreWFBucket(bucket)
     ensures |bucket.keys| <= WeightBucket(bucket)
-    ensures |bucket.b| <= WeightBucket(bucket)
     decreases bucket.keys
   {
     KeyMultisetLeWeight(multiset(bucket.keys));
@@ -1621,13 +620,12 @@ module BucketWeights {
 
   // used
   lemma WeightBucketListOneEmpty()
-  ensures WeightBucketList([B(map[])]) == 0
+  ensures WeightBucketList([EmptyBucket()]) == 0
   {
     reveal_WeightBucketList();
     WeightBucketEmpty();
   }
 
-  
   // used
   lemma WeightBucketLeBucketList(blist: BucketList, i: int)
   requires 0 <= i < |blist|
@@ -1645,47 +643,83 @@ module BucketWeights {
     }
   }
 
-  // used internally
-  lemma WMWeightBucketListInsert(blist: BucketList, pivots: PivotTable, key: Key, msg: Message)
-    requires WFBucketList(blist, pivots)
-    requires BoundedKey(pivots, key)
-    requires BucketWellMarshalled(blist[Route(pivots, key)])
-    ensures WeightBucketList(BucketListInsert(blist, pivots, key, msg)) <=
-    WeightBucketList(blist) + WeightKey(key) + WeightMessage(msg)
+  lemma WeightBucketInsert(bucket: Bucket, key: Key, msg: Message)
+  requires PreWFBucket(bucket)
+  ensures WeightBucket(BucketInsert(bucket, key, msg)) <=
+      WeightBucket(bucket) + WeightKey(key) + WeightMessage(msg)
   {
-    var i := Route(pivots, key);
-    var bucket := blist[i];
-
-    var mergedMsg := Merge(msg, BucketGet(bucket, key));
-    var mergedWeight := if mergedMsg != IdentityMessage() then WeightKey(key) + WeightMessage(mergedMsg) else 0;
-
-    calc {
-      WeightBucket(BucketInsert(bucket, key, msg));
-        { KeyContribution(BucketInsert(bucket, key, msg), key); }
-      WeightBucket(Image(BucketInsert(bucket, key, msg), ExcludeKey(key))) + WeightOneKey(BucketInsert(bucket, key, msg), key);
+    var mergedMsg := Merge(msg, BucketGet(bucket.as_map(), key));
+    if mergedMsg == IdentityMessage() {
+      // case 1: entry from map is removed
+      calc <= {
+        WeightBucket(BucketInsert(bucket, key, msg));
+        WeightBucket(B(MapRemove1(bucket.as_map(), key)));
         {
-          ImageShape(BucketInsert(bucket, key, msg), ExcludeKey(key));
-          ImageShape(bucket, ExcludeKey(key));
-          WellMarshalledBucketsEq(Image(BucketInsert(bucket, key, msg), ExcludeKey(key)), Image(bucket, ExcludeKey(key)));
+         Weight_Bucket_eq_BucketMap(MapRemove1(bucket.as_map(), key));
         }
-      WeightBucket(Image(bucket, ExcludeKey(key))) + WeightOneKey(BucketInsert(bucket, key, msg), key);
-      WeightBucket(Image(bucket, ExcludeKey(key))) + mergedWeight;
-    }
-
-    calc {
-      WeightBucketList(BucketListInsert(blist, pivots, key, msg));
-        { WeightBucketListReplace(blist, i, BucketInsert(bucket, key, msg)); }
-      WeightBucketList(blist) - WeightBucket(bucket) + WeightBucket(BucketInsert(bucket, key, msg));
-        // Calc above
-      WeightBucketList(blist) - WeightBucket(bucket) + WeightBucket(Image(bucket, ExcludeKey(key))) + mergedWeight;
-        { KeyContribution(bucket, key); }
-      WeightBucketList(blist) - (WeightBucket(Image(bucket, ExcludeKey(key))) + WeightOneKey(bucket, key))
-        + WeightBucket(Image(bucket, ExcludeKey(key))) + mergedWeight;
-      <= // terms cancel; mergedWeight definition
-      WeightBucketList(blist) - WeightOneKey(bucket, key) + WeightKey(key) + WeightMessage(mergedMsg);
-      <=
-        { MergeGainsNoWeight(msg, BucketGet(bucket, key)); }
-      WeightBucketList(blist) + WeightKey(key) + WeightMessage(msg);
+        WeightBucketMap(MapRemove1(bucket.as_map(), key));
+        {
+          WeightBucketMapSubsetLe(MapRemove1(bucket.as_map(), key), bucket.as_map());
+        }
+        WeightBucketMap(bucket.as_map());
+        {
+          Weight_BucketMap_le_Bucket(bucket);
+        }
+        WeightBucket(bucket);
+        WeightBucket(bucket) + WeightKey(key) + WeightMessage(msg);
+      }
+    } else if key !in bucket.as_map() {
+      // case 2: entry inserted into map
+      calc <= {
+        WeightBucket(BucketInsert(bucket, key, msg));
+        WeightBucket(B(bucket.as_map()[key := mergedMsg]));
+        {
+          Weight_Bucket_eq_BucketMap(bucket.as_map()[key := mergedMsg]);
+        }
+        WeightBucketMap(bucket.as_map()[key := mergedMsg]);
+        {
+          WeightBucketInduct(bucket.as_map(), key, mergedMsg);
+        }
+        WeightBucketMap(bucket.as_map()) + WeightKey(key) + WeightMessage(mergedMsg);
+        WeightBucketMap(bucket.as_map()) + WeightKey(key) + WeightMessage(msg);
+        {
+          Weight_BucketMap_le_Bucket(bucket);
+        }
+        WeightBucket(bucket) + WeightKey(key) + WeightMessage(msg);
+      }
+    } else {
+      // case 3: entry is replaced
+      // relies on weight(mergedMsg) <= weight(oldMsg) + weight(msg)
+      var m' := MapRemove1(bucket.as_map(), key);
+      var oldMsg := bucket.as_map()[key];
+      calc <= {
+        WeightBucket(BucketInsert(bucket, key, msg));
+        {
+          assert m'[key := mergedMsg] == bucket.as_map()[key := mergedMsg];
+        }
+        WeightBucket(B(m'[key := mergedMsg]));
+        {
+          Weight_Bucket_eq_BucketMap(m'[key := mergedMsg]);
+        }
+        WeightBucketMap(m'[key := mergedMsg]);
+        {
+          WeightBucketInduct(m', key, mergedMsg);
+        }
+        WeightBucketMap(m') + WeightKey(key) + WeightMessage(mergedMsg);
+        WeightBucketMap(m') + WeightKey(key) + WeightMessage(oldMsg) + WeightMessage(msg);
+        {
+          WeightBucketInduct(m', key, oldMsg);
+        }
+        WeightBucketMap(m'[key := oldMsg]) + WeightMessage(msg);
+        {
+          assert m'[key := oldMsg] == bucket.as_map();
+        }
+        WeightBucketMap(bucket.as_map()) + WeightMessage(msg);
+        {
+          Weight_BucketMap_le_Bucket(bucket);
+        }
+        WeightBucket(bucket) + WeightKey(key) + WeightMessage(msg);
+      }
     }
   }
 
@@ -1697,52 +731,17 @@ module BucketWeights {
   {
     var i := Route(pivots, key);
     var bucket := blist[i];
-    var wmbucket := Image(bucket, AllKeys());
-    var blist' := blist[i := wmbucket];
+    var bucket' := BucketInsert(bucket, key, msg);
 
-    ImageMapIdentity(bucket, AllKeys());
-    WeightWellMarshalledLe(bucket, wmbucket);
-    assert BucketListInsert(blist', pivots, key, msg) == BucketListInsert(blist, pivots, key, msg);
-  
-    WeightWellMarshalledListPointwiseLe(blist, blist');
-    WMWeightBucketListInsert(blist', pivots, key, msg);
+    calc <= {
+      WeightBucketList(BucketListInsert(blist, pivots, key, msg));
+        { WeightBucketListReplace(blist, i, BucketInsert(bucket, key, msg)); }
+      WeightBucketList(blist) - WeightBucket(bucket) + WeightBucket(BucketInsert(bucket, key, msg));
+        { WeightBucketInsert(bucket, key, msg); }
+      WeightBucketList(blist) + WeightKey(key) + WeightMessage(msg);
+    }
   }
   
-  
-  // used
-  lemma WeightBucketIntersect(bucket: Bucket, keys: set<Key>)
-    requires PreWFBucket(bucket)
-    ensures WeightBucket(BucketIntersect(bucket, keys)) <= WeightBucket(bucket)
-  {
-    var wmbucket := Image(bucket, AllKeys());
-    var ikeys := iset k | k in keys;
-    ImageMapIdentity(bucket, AllKeys());
-    WeightWellMarshalledLe(bucket, wmbucket);
-
-    reveal_BucketIntersect();
-    ImageShape(wmbucket, ikeys);
-    WellMarshalledBucketsEq(BucketIntersect(wmbucket, keys), Image(wmbucket, ikeys));
-    ImageIdentity(wmbucket, AllKeys());
-    WeightBucketSubset(wmbucket, ikeys, AllKeys());
-  }
-
-  // used
-  lemma WeightBucketComplement(bucket: Bucket, keys: set<Key>)
-    requires PreWFBucket(bucket)
-    ensures WeightBucket(BucketComplement(bucket, keys)) <= WeightBucket(bucket)
-  {
-    var wmbucket := Image(bucket, AllKeys());
-    var ikeys := iset k | k !in keys;
-    ImageMapIdentity(bucket, AllKeys());
-    WeightWellMarshalledLe(bucket, wmbucket);
-
-    reveal_BucketComplement();
-    ImageShape(wmbucket, ikeys);
-    WellMarshalledBucketsEq(BucketComplement(wmbucket, keys), Image(wmbucket, ikeys));
-    ImageIdentity(wmbucket, AllKeys());
-    WeightBucketSubset(wmbucket, ikeys, AllKeys());
-  }
-
   lemma WeightKeyListAdditive(a: seq<Key>, b: seq<Key>)
   ensures WeightKeyList(a) + WeightKeyList(b) == WeightKeyList(a + b)
   {
@@ -1787,4 +786,21 @@ module BucketWeights {
     WeightMessageSingleton(msg);
   }
 
+  lemma WeightBucketMapSingleton(key: Key, msg: Message)
+  ensures WeightBucketMap(map[key := msg])
+      == WeightKey(key) + WeightMessage(msg)
+  {
+    var m := map[];
+    assert map[key := msg] == m[key := msg];
+    calc {
+      WeightBucketMap(map[key := msg]);
+      WeightBucketMap(m[key := msg]);
+      { WeightBucketInduct(m, key, msg); }
+      WeightBucketMap(m) + WeightKey(key) + WeightMessage(msg);
+      {
+        assert WeightBucketMap(map[]) == 0 by { reveal_WeightBucketMap(); }
+      }
+      WeightKey(key) + WeightMessage(msg);
+    }
+  }
 }
